Consider the given expression, <br />     ${{S}_{n}}=\frac{1}{1+\sqrt{n}}+\frac{1}{2+\sqrt{2n}}+\ldots +\frac{1}{n+\sqrt{{{n}^{2}}}}$ <br />This can be converted to summation as, <br />     $${{S}_{n}}=\underset{r=1}{\overset{n}{\mathop \sum }}\, \frac{1}{r+\sqrt{rn}}$$<br /> Now we will apply limits, we get<br />     $\underset{n\to \infty }{\mathop{\lim }}\, {{S}_{n}}=\underset{n\to \infty }{\mathop{\lim }}\, \underset{r=1}{\overset{n}{\mathop \sum }}\, \frac{1}{r+\sqrt{rn}}$ <br />Dividing numerator and denominator by  n, we get<br />     $\underset{n\to \infty }{\mathop{\lim }}\, {{S}_{n}}=\underset{n\to \infty }{\mathop{\lim }}\, \underset{r=1}{\overset{n}{\mathop \sum }}\, \frac{\frac{1}{n}}{\frac{\left( r+\sqrt{rn} \right)}{n}}$ <br />     $\Rightarrow \underset{n\to \infty }{\mathop{\lim }}\, {{S}_{n}}=\underset{n\to \infty }{\mathop{\lim }}\, \underset{r=1}{\overset{n}{\mathop \sum }}\, \frac{\frac{1}{n}}{\frac{r}{n}+\frac{\sqrt{rn}}{n}}$ <br />     $\Rightarrow \underset{n\to \infty }{\mathop{\lim }}\, {{S}_{n}}=\underset{n\to \infty }{\mathop{\lim }}\, \underset{r=1}{\overset{n}{\mathop \sum }}\, \frac{\frac{1}{n}}{\frac{r}{n}+\sqrt{\frac{rn}{{{n}^{2}}}}}$ <br />     $\Rightarrow \underset{n\to \infty }{\mathop{\lim }}\, {{S}_{n}}=\underset{n\to \infty }{\mathop{\lim }}\, \underset{r=1}{\overset{n}{\mathop \sum }}\, \frac{\frac{1}{n}}{\frac{r}{n}+\sqrt{\frac{r}{n}}}\ldots \ldots \left( i \right)$ $$$$ <br />Now let, <br />     $\frac{r}{n}=x\Rightarrow \frac{1}{n}=dx$ <br />Let’s find the limits, <br />When $$r=1\Rightarrow x=0$$<br />When $r=n\Rightarrow x=1$ <br />Considering these values the summation can be written as integral form. We get, <br />     $\underset{r=1}{\overset{n}{\mathop \sum }}\, \frac{\frac{1}{n}}{\frac{r}{n}+\sqrt{\frac{r}{n}}}=\underset{0}{\overset{1}{\mathop \int }}\, \frac{dx}{x+\sqrt{x}}\ldots \ldots \ldots \left( ii \right)$ <br />Now we will find the integration as follows:<br />     $\underset{0}{\overset{1}{\mathop \int }}\, \frac{dx}{x+\sqrt{x}}=\underset{0}{\overset{1}{\mathop \int }}\, \frac{dx}{\sqrt{x}\left( \sqrt{x}+1 \right)}\ldots \ldots .\left( iii \right)$ <br />Let’s substitute, <br />     $u=\sqrt{x}+1$ <br />Differentiating, we get<br />     $du=\frac{1}{2\sqrt{x}}dx\Rightarrow dx=2\sqrt{x}du$ <br />Substituting these values in equation (iii), we get<br />     $\underset{0}{\overset{1}{\mathop \int }}\, \frac{dx}{x+\sqrt{x}}=\underset{0}{\overset{1}{\mathop \int }}\, \frac{2\sqrt{x}du}{\sqrt{x}\left( u \right)}$ <br />     $\underset{0}{\overset{1}{\mathop \int }}\, \frac{dx}{x+\sqrt{x}}=2\underset{0}{\overset{1}{\mathop \int }}\, \frac{1}{u}du$ <br />But we know, $\mathop{\int }^{}\frac{1}{u}=\ln u$ , so above equation becomes, <br />     $\underset{0}{\overset{1}{\mathop \int }}\, \frac{dx}{x+\sqrt{x}}=2\left[ lnu \right]_{0}^{1}$ <br />Substituting back the value of u, we get<br />     $\underset{0}{\overset{1}{\mathop \int }}\, \frac{dx}{x+\sqrt{x}}=2\left[ \ln (\sqrt{x}+1) \right]_{0}^{1}$ <br />Applying the upper and lower bounds, we get<br />     $\underset{0}{\overset{1}{\mathop \int }}\, \frac{dx}{x+\sqrt{x}}=2\left[ \ln (\sqrt{1}+1 \right)\left] -2 \right[\ln (\sqrt{0}+1)]$ <br />     $\underset{0}{\overset{1}{\mathop \int }}\, \frac{dx}{x+\sqrt{x}}=2\left[ \ln 2\left] -2 \right[\ln (1 \right)]$ <br />But we know, $ln1=0$, so we get<br />     $\underset{0}{\overset{1}{\mathop \int }}\, \frac{dx}{x+\sqrt{x}}=2\left[ ln2 \right]-0$ <br />     $\underset{0}{\overset{1}{\mathop \int }}\, \frac{dx}{x+\sqrt{x}}=\left[ \ln {{2}^{2}} \right]=\ln 4$ <br />Substituting this in equation (ii), we get<br />     $\underset{r=1}{\overset{n}{\mathop \sum }}\, \frac{\frac{1}{n}}{\frac{r}{n}+\sqrt{\frac{r}{n}}}=\ln 4$ <br />Substituting this value in equation (i), we get<br />     $\Rightarrow \underset{n\to \infty }{\mathop{\lim }}\, {{S}_{n}}=\underset{n\to \infty }{\mathop{\lim }}\, \ln 4$ <br />As the RHS is free of variable, so we can remove the limit, so we get<br />     $\Rightarrow \underset{n\to \infty }{\mathop{\lim }}\, {{S}_{n}}=\ln 4$ <br />Note:  The possibility for the mistake is that in the following equation, <br />     $\Rightarrow \underset{n\to \infty }{\mathop{\lim }}\, {{S}_{n}}=\underset{n\to \infty }{\mathop{\lim }}\, \underset{r=1}{\overset{n}{\mathop \sum }}\, \frac{\frac{1}{n}}{\frac{r}{n}+\sqrt{\frac{rn}{{{n}^{2}}}}}$ <br />we see that the n2 term becomes ‘n’ when taken out of the square root.<br />So, instead of dividing by n2 we can just divide the ‘r’ by ‘n’ and we won’t get the same answer.<br /><br /><br />
